Remove old sequential code (#593)
* remove old sequential files

* rename duplicate files

* fix imports

* fix build errors

* fix imports in silveroak-opentitan and remove Cipher.v

* rename CipherNewLoop => CipherCircuit

* fix build errors and re-generate assumption-tracking files

* remove Sequential from Cava2HDL.cabal

acorn-examples/AdderTree.v
@@ -29,7 +29,7 @@ Require Import ExtLib.Structures.Monads.
 Export MonadNotation.
 
 Require Import Cava.Cava.
-Require Import Cava.Acorn.AcornNew.
+Require Import Cava.Acorn.Acorn.
 Require Import Cava.Lib.UnsignedAdders.
 
 Existing Instance CombinationalSemantics.
@@ -78,17 +78,15 @@ Local Open Scope string_scope.
 Local Open Scope vector_scope.
 
 Definition v0_v1 := [v0; v1].
-Definition v0_plus_v1 : list (Bvector 8) := unIdent (adderTree 0 [v0_v1]%list).
+Definition v0_plus_v1 : Bvector 8 := unIdent (adderTree 0 v0_v1).
 
-Example sum_vo_v1 : unIdent (adderTree2 [v0_v1]%list) = [N2Bv_sized 8 21]%list.
+Example sum_vo_v1 : unIdent (adderTree2 v0_v1) = N2Bv_sized 8 21.
 Proof. reflexivity. Qed.
 
-
-
 Definition v0_3 := [v0; v1; v2; v3].
-Definition sum_v0_3 : list (Bvector 8) := unIdent (adderTree4 [v0_3]%list).
+Definition sum_v0_3 : Bvector 8 := unIdent (adderTree4 v0_3).
 
-Example sum_v0_v1_v2_v3 : unIdent (adderTree4 [v0_3]%list) = [N2Bv_sized 8 30]%list.
+Example sum_v0_v1_v2_v3 : unIdent (adderTree4 v0_3) = N2Bv_sized 8 30.
 Proof. reflexivity. Qed.
 
 Definition adder_tree_Interface name nrInputs bitSize
