acorn-examples/Examples.v
@@ -17,7 +17,7 @@
 (* Experiments with the primitives that form the core of Cava. *)
 
 Require Import Coq.Lists.List.
-Require Import Cava.Acorn.AcornNew.
+Require Import Cava.Acorn.Acorn.
 Import ListNotations.
 
 (* Experiments with the primitive Cava gates. *)
