acorn-examples/xilinx/XilinxAdderExamples.v
@@ -24,6 +24,7 @@ Require Import ExtLib.Structures.Monads.
 Require Import Cava.Cava.
 Require Import Cava.Acorn.Acorn.
 Require Import Cava.Acorn.XilinxAdder.
+Existing Instance CavaCombinationalNet.
 
 (****************************************************************************)
 (* A few tests to check the unsigned adder.        *)
@@ -42,24 +43,24 @@ Definition v44  := N2Bv_sized 8 44.
 
 (* Perform a few basic checks to make sure the adder works. *)
 
-Example xadd_17_52_0 : combinational (xilinxAdderWithCarry ([false], ([v17], [v52]))) =
-                                     ([v69], [false]).
+Example xadd_17_52_0 : unIdent (xilinxAdderWithCarry (false, (v17, v52))) =
+                       (v69, false).
 Proof. reflexivity. Qed.
 
-Example xadd_17_52_1 : combinational (xilinxAdderWithCarry ([true], ([v17], [v52]))) =
-                                     ([v70], [false]).
+Example xadd_17_52_1 : unIdent (xilinxAdderWithCarry (true, (v17, v52))) =
+                       (v70, false).
 Proof. reflexivity. Qed.
 
-Example xadd_1_255_1 : combinational (xilinxAdderWithCarry ([false], ([v1], [v255]))) =
-                                     ([v0], [true]).
+Example xadd_1_255_1 : unIdent (xilinxAdderWithCarry (false, (v1, v255))) =
+                       (v0, true).
 Proof. reflexivity. Qed.
 
-Example xadd_0_255_1 : combinational (xilinxAdderWithCarry ([true], ([v0], [v255]))) =
-                                     ([v0], [true]).
+Example xadd_0_255_1 : unIdent (xilinxAdderWithCarry (true, (v0, v255))) =
+                       (v0, true).
 Proof. reflexivity. Qed.
 
-Example xadd_200_100_0 : combinational (xilinxAdderWithCarry ([false], ([v200], [v100]))) =
-                                       ([v44], [true]).
+Example xadd_200_100_0 : unIdent (xilinxAdderWithCarry (false, (v200, v100))) =
+                         (v44, true).
 Proof. reflexivity. Qed.
 
 (****************************************************************************)
@@ -95,10 +96,7 @@ Definition adder8_tb_inputs :=
    (1, (255, 255))].
 
 Definition adder8_tb_expected_outputs :=
-  map (fun '(i0,i1,i2) =>
-         let '(r1,r2) := combinational (xilinxAdderWithCarryFlat ([i0],[i1],[i2])%list) in
-         (List.hd (defaultCombValue _) r1, List.hd (defaultCombValue _) r2))
-      adder8_tb_inputs.
+  multistep (Comb xilinxAdderWithCarryFlat) adder8_tb_inputs.
 
 Definition adder8_tb :=
   testBench "adder8_tb" adder8Interface
