cava/Cava/Acorn/CavaClass.v
@@ -92,26 +92,3 @@ Class Cava (signal : SignalType -> Type) := {
              tupleInterface signal (map port_type (circuitInputs intf)) ->
              cava (tupleInterface signal ((map port_type (circuitOutputs intf))));
 }.
-
-(* Sequential semantics -- assumes the sequential part of the interpretation is in [signal] *)
-Class CavaSeq {signal : SignalType -> Type} (combinationalSemantics : Cava signal) := {
-  (* A unit delay with a reset value. *)
-  delayWith : forall {t: SignalType}, combType t -> signal t -> cava (signal t);
-  (* A unit delay with a clock-enable input. *)
-  delayEnableWith : forall {t: SignalType}, combType t -> signal Bit -> signal t -> cava (signal t);
-  (* Feedback loop, with unit delay inserted into the feedback path and current
-     state available at output . *)
-  loopDelaySR : forall {A B: SignalType},
-                combType B ->
-                (signal A * signal B -> cava (signal B)) ->
-                signal A ->
-                cava (signal B);
-  (* A version of loopDelayEnable with a clock enable and current state at
-     the output. *)
-  loopDelaySEnableR : forall {A B: SignalType},
-                      combType B ->
-                      signal Bit -> (* Clock enable *)
-                      (signal A * signal B -> cava (signal B)) ->
-                      signal A ->
-                      cava (signal B);
-}.
