cava/Cava/Acorn/Identity.v
@@ -1,5 +1,5 @@
 (****************************************************************************)
-(* Copyright 2020 The Project Oak Authors                                   *)
+(* Copyright 2021 The Project Oak Authors                                   *)
 (*                                                                          *)
 (* Licensed under the Apache License, Version 2.0 (the "License")           *)
 (* you may not use this file except in compliance with the License.         *)
@@ -26,13 +26,12 @@ Require Import Cava.ListUtils.
 Require Import Cava.VectorUtils.
 Require Import Cava.Lib.BitVectorOps.
 Require Import Cava.Acorn.CavaClass.
-Require Import Cava.Acorn.CombinationalMonad.
+Require Import Cava.Acorn.Combinational.
 Require Import Cava.Acorn.Combinators.
 Import VectorNotations ListNotations.
 Open Scope list_scope.
 
 Existing Instance CombinationalSemantics.
-
 
 Section MapT.
   Lemma mapT_vector_ident {A B n} (f : A -> ident B) (v : Vector.t A n) :
@@ -57,135 +56,16 @@ Section MapT.
     simpl. rewrite IHl. reflexivity.
   Qed.
 End MapT.
-Hint Rewrite @mapT_vector_ident @mapT_vident @mapT_lident using solve [eauto] : simpl_ident.
-
-Section PeelUnpeel.
-  Lemma peelVecList_cons_cons {A n} (a : combType A) (v : combType (Vec A n)) :
-    peelVecList [(a :: v)%vector] = ([a]%list :: peelVecList [v])%vector.
-  Proof.
-    cbv [peelVecList indexConstBoolList]. cbn [List.map Vector.map].
-    apply to_list_inj. autorewrite with push_to_list.
-    rewrite <-cons_seq, <-seq_shift. cbn [List.map]. rewrite List.map_map.
-    cbn. autorewrite with natsimpl.
-    reflexivity.
-  Qed.
-
-  (* Useful for unpeel *)
-  Lemma max_length_same_length {A n} (v : Vector.t (list A) n) m len:
-    (forall l, InV l v -> length l = len) -> n <> 0 -> m <= len ->
-    fold_left PeanoNat.Nat.max m (map (@length _) v) = len.
-  Proof.
-    revert m; induction n; intros; [ congruence | ].
-    rewrite (eta v) in *. cbn [Vector.map InV] in *.
-    autorewrite with vsimpl in *.
-    destruct (PeanoNat.Nat.eq_dec n 0);
-      subst; autorewrite with push_vector_fold vsimpl;
-        repeat match goal with
-               | Hin : forall l, _ -> length l = _ |- _ =>
-                 rewrite Hin by (tauto || lia)
-               | _ => rewrite IHn; [ | intros; try lia .. ]
-               | _ => reflexivity
-               | _ => lia
-               end.
-  Qed.
-
-  Lemma peelVecList_length {A n} (v : seqType (Vec A n)) l :
-    InV l (peelVecList v) -> length l = length v.
-  Proof.
-    cbv [peelVecList indexConstBoolList].
-    rewrite InV_map_iff. destruct 1 as [? [? ?]].
-    subst. autorewrite with push_length. reflexivity.
-  Qed.
-
-  Lemma unpeelVecList_cons_singleton {A n} (a : combType A) (v : Vector.t (seqType A) n) x :
-    (forall l, InV l v -> length l = 1) -> n <> 0 -> unpeelVecList v = [x]%list ->
-    unpeelVecList ([a]%list :: v)%vector = [(a :: x)%vector].
-  Proof.
-    cbv [unpeelVecList]; intros Hin ? Heq.
-    rewrite max_length_same_length with (len:=1) in Heq by (lia || eauto).
-    rewrite max_length_same_length with (len:=1)
-      by (try lia; eauto; intros *; rewrite InV_cons_iff;
-          destruct 1; subst; intros; eauto).
-    cbn [List.map List.seq Vector.map List.nth] in *.
-    inversion Heq; reflexivity.
-  Qed.
-End PeelUnpeel.
-
-(* Lemmas about combinators specialized to the identity monad *)
-Section Combinators.
-  Lemma zipWith_unIdent {A B C : SignalType} n
-        (f : seqType A * seqType B -> cava (seqType C))
-        (spec : combType A -> combType B -> combType C)
-        (va : combType (Vec A n)) (vb : combType (Vec B n)) :
-    n <> 0 ->
-    (forall a b, unIdent (f ([a], [b])) = [spec a b]) ->
-    unIdent (@zipWith _ _ A B C n f [va] [vb])
-    = [Vector.map2 spec va vb].
-  Proof.
-    cbv [zipWith Traversable.mapT Traversable_vector].
-    cbn [peel unpeel monad CombinationalSemantics].
-    cbn [bind ret Monad_ident unIdent] in *.
-    rewrite mapT_vector_ident.
-    revert va vb; induction n; intros; [ lia | ].
-    { rewrite (eta va), (eta vb).
-      autorewrite with push_vcombine push_vector_map vsimpl.
-      cbn [combType]  in *. rewrite !peelVecList_cons_cons.
-      autorewrite with push_vcombine push_vector_map vsimpl.
-      lazymatch goal with
-      | Hspec : context [unIdent (f _)] |- _ =>
-        rewrite Hspec
-      end.
-      fold combType.
-      destruct (PeanoNat.Nat.eq_dec n 0).
-      { subst n. eapply case0 with (v:=Vector.tl va).
-        eapply case0 with (v:=Vector.tl vb).
-        reflexivity. }
-      cbv [seqType].
-      erewrite unpeelVecList_cons_singleton; eauto; [ ].
-      intros *. rewrite InV_map_iff.
-      destruct 1 as [? [? ?]].
-      subst.
-      cbv [vcombine] in *.
-      repeat match goal with
-             | H : _ |- _ =>
-               apply InV_map2_impl in H; destruct H as [? [? [? [? ?]]]]; subst
-             | H : InV _ _ |- _ => apply peelVecList_length in H
-             end.
-      match goal with
-      | |- context [f (?l1, ?l2)] =>
-        destruct l1 as [| ? [|? ?] ];
-          destruct l2 as [| ? [|? ?] ];
-          cbn [length] in *; try lia
-      end.
-      lazymatch goal with
-      | Hspec : context [unIdent (f _)] |- _ =>
-        rewrite Hspec
-      end.
-      reflexivity. }
-  Qed.
-End Combinators.
-
-
-Section Vectors.
-  Lemma xorV_unIdent n a b :
-    n <> 0 ->
-    unIdent (@xorV _ _ n ([a],[b])) = [Vector.map2 xorb a b].
-  Proof.
-    intros. cbv [xorV]. cbn [fst snd].
-    erewrite zipWith_unIdent; [ reflexivity | lia | ].
-    intros; reflexivity.
-  Qed.
-End Vectors.
 
 Instance MonadLaws_ident : MonadLaws Monad_ident.
 Proof. econstructor; intros; exact eq_refl. Defined.
 
 (* Automation to help simplify expressions using the identity monad *)
 Create HintDb simpl_ident discriminated.
-Hint Rewrite @zipWith_unIdent @xorV_unIdent
-     using solve [eauto]: simpl_ident.
+Hint Rewrite @mapT_vector_ident @mapT_vident @mapT_lident using solve [eauto] : simpl_ident.
 Ltac simpl_ident :=
   repeat
     first [ progress autorewrite with simpl_ident
           | progress cbn [fst snd bind ret Monad_ident monad
+                              peel unpeel constant
                               CombinationalSemantics unIdent] ].
