cava/Cava/Acorn/XilinxAdder.v
@@ -74,26 +74,25 @@ Section WithCombinational.
 
   (* A quick sanity check of the Xilinx adder with carry in and out *)
   Example xilinx_add_17_52:
-    combinational (xilinxAdderWithCarry
-                  ([false], ([N2Bv_sized 8 17], [N2Bv_sized 8 52]))) =
-                  ([N2Bv_sized 8 69], [false]).
+    unIdent (xilinxAdderWithCarry
+                  (false, (N2Bv_sized 8 17, N2Bv_sized 8 52))) =
+                  (N2Bv_sized 8 69, false).
   Proof. vm_compute. reflexivity. Qed.
 
   (* A quick sanity check of the Xilinx adder with no bit-growth *)
   Example xilinx_no_growth_add_17_52:
-    combinational (xilinxAdder [N2Bv_sized 8 17] [N2Bv_sized 8 52]) =
-                  [N2Bv_sized 8 69].
+    unIdent (xilinxAdder (N2Bv_sized 8 17) (N2Bv_sized 8 52)) =
+                  (N2Bv_sized 8 69).
   Proof. reflexivity. Qed.
 
   (* A proof that the the full-adder is correct. *)
   Lemma xilinxFullAdder_behaviour :
     forall (a : bool) (b : bool) (cin : bool),
-          combinational (xilinxFullAdder ([cin], ([a], [b])))
-          = ([xorb cin (xorb a b)],
-             [(a && b) || (b && cin) || (a && cin)]).
+          unIdent (xilinxFullAdder (cin, (a, b)))
+          = (xorb cin (xorb a b),
+             (a && b) || (b && cin) || (a && cin)).
   Proof.
     intros.
-    unfold combinational.
     unfold fst.
     simpl.
     case a, b, cin.
