silveroak-opentitan/aes/Acorn/AESExtraction.v
@@ -15,8 +15,8 @@
 (****************************************************************************)
 
 Require Import AcornAes.Pkg.
-Require Import AcornAes.Cipher.
-Require Import AcornAes.CipherNewLoop.
+Require Import AcornAes.CipherCircuit.
+Require Import AcornAes.CipherCircuit.
 Require Import AcornAes.MixColumnsCircuit.
 Require Import AcornAes.ShiftRowsCircuit.
 Require Import AcornAes.SubBytesCircuit.
@@ -37,8 +37,7 @@ Require Import RecordUpdate.RecordSet.
 Extraction Language Haskell.
 
 Extraction Library Pkg.
-Extraction Library Cipher.
-Extraction Library CipherNewLoop.
+Extraction Library CipherCircuit.
 Extraction Library MixColumnsCircuit.
 Extraction Library ShiftRowsCircuit.
 Extraction Library SubBytesCircuit.
