silveroak-opentitan/aes/Acorn/AddRoundKeyEquivalence.v
@@ -20,8 +20,7 @@ Require Import ExtLib.Structures.Monads.
 Require Import Cava.ListUtils.
 Require Import Cava.Tactics.
 Require Import Cava.VectorUtils.
-Require Import Cava.Acorn.MonadFacts.
-Require Import Cava.Acorn.IdentityNew.
+Require Import Cava.Acorn.Identity.
 Require Import Cava.Acorn.Acorn.
 Require Import Cava.Lib.BitVectorOps.
 Import ListNotations.
