silveroak-opentitan/aes/Acorn/CipherControlCircuit.v
@@ -35,8 +35,9 @@ Require Import AcornAes.SubBytesCircuit.
 Require Import AcornAes.AddRoundKeyCircuit.
 Require Import AcornAes.ShiftRowsCircuit.
 Require Import AcornAes.MixColumnsCircuit.
-Require Import AcornAes.CipherNewLoop.
+Require Import AcornAes.CipherCircuit.
 Import Circuit.Notations.
+Existing Instance CavaCombinationalNet.
 
 Require Import AcornAes.ShiftRowsNetlist.
 Require Import AcornAes.MixColumnsNetlist.
@@ -49,7 +50,6 @@ Notation round_index := (Vec Bit 4) (only parsing).
 
 Section WithCava.
   Context {signal} {semantics : Cava signal}.
-  Context {seqsemantics : CavaSeq semantics}.
 
   Local Infix "==?" := eqb (at level 40).
 
@@ -91,7 +91,7 @@ Section WithCava.
     Definition inv_mix_columns_key := aes_mix_columns' (constant true).
 
     (* Plug in our concrete components to the skeleton in Cipher.v *)
-    Definition cipher := CipherNewLoop.cipher
+    Definition cipher := CipherCircuit.cipher
       aes_sub_bytes' aes_shift_rows' aes_mix_columns' aes_add_round_key
       inv_mix_columns_key key_expand.
   End PkgNotations.
