silveroak-opentitan/aes/Acorn/MixColumnsNetlist.v
@@ -44,7 +44,8 @@ Local Open Scope list_scope.
 
 (* Compute the expected outputs from the Coq/Cava semantics. *)
 Definition aes_mix_cols_expected_outputs :=
-  combinational (aes_mix_columns [false] [fromNatVec test_state]).
+  multistep (Comb (fun '(op_i, data_i) => aes_mix_columns op_i data_i))
+            [(false, fromNatVec test_state)].
 
 Definition aes_mix_columns_tb :=
   testBench "aes_mix_columns_tb"
