tests/Array.v
@@ -24,7 +24,7 @@ Require Import ExtLib.Structures.Monads.
 Export MonadNotation.
 
 Require Import Cava.Cava.
-Require Import Cava.Acorn.AcornNew.
+Require Import Cava.Acorn.Acorn.
 Require Import Cava.Lib.UnsignedAdders.
 Require Import Coq.Vectors.Vector.
 Require Import Cava.VectorUtils.
