tests/xilinx/LUTTests.v
@@ -22,6 +22,7 @@ Require Import ExtLib.Structures.Monads.
 
 Require Import Cava.Cava.
 Require Import Cava.Acorn.Acorn.
+Existing Instance CavaCombinationalNet.
 
 Section WithCava.
   Context {signal} `{Cava signal}.
@@ -52,7 +53,7 @@ Section WithCava.
               andb (andb (andb (andb i0 i1) (andb i2 i3)) i4) i5) i ;;
     ret o.
 
-End WithCava.  
+End WithCava.
 
 (******************************************************************************)
 (* LUT1 config test                                                           *)
@@ -66,8 +67,7 @@ End WithCava.
   Definition lut1_inv_tb_inputs := [false; true].
 
   Definition lut1_inv_tb_expected_outputs : list bool :=
-    map (fun i => List.hd (defaultCombValue _) (combinational (lut1_inv [i]%list)))
-        lut1_inv_tb_inputs.
+    multistep (Comb lut1_inv) lut1_inv_tb_inputs.
 
   Definition lut1_inv_tb :=
     testBench "lut1_inv_tb" lut1_inv_Interface
@@ -88,9 +88,8 @@ Definition lut2_and_nelist := makeNetlist lut2_and_Interface lut2_and.
 Definition lut2_and_tb_inputs : list (bool * bool) :=
  [(false, false); (false, true); (true, false); (true, true)].
 
- Definition lut2_and_tb_expected_outputs : list bool :=
-   map (fun '(i0,i1) => List.hd (defaultCombValue _)
-                             (combinational (lut2_and ([i0],[i1])%list))) lut2_and_tb_inputs.
+Definition lut2_and_tb_expected_outputs : list bool :=
+  multistep (Comb lut2_and) lut2_and_tb_inputs.
 
 Definition lut2_and_tb :=
   testBench "lut2_and_tb" lut2_and_Interface
@@ -116,10 +115,8 @@ Definition lut3_mux_tb_inputs : list (bool * bool * bool) :=
   (true, true, false);
   (true, true, true)].
 
- Definition lut3_mux_tb_expected_outputs : list bool :=
-   map (fun '(i0,i1,i2) =>
-          List.hd (defaultCombValue _) (combinational (lut3_mux ([i0],[i1],[i2])%list)))
-       lut3_mux_tb_inputs.
+Definition lut3_mux_tb_expected_outputs : list bool :=
+  multistep (Comb lut3_mux) lut3_mux_tb_inputs.
 
 Definition lut3_mux_tb :=
   testBench "lut3_mux_tb" lut3_mux_Interface
@@ -145,10 +142,7 @@ Definition lut4_and_tb_inputs : list (bool * bool * bool * bool) :=
   (true, true, true, true)].
 
 Definition lut4_and_tb_expected_outputs : list bool :=
-  map (fun '(i0,i1,i2,i3) =>
-         List.hd (defaultCombValue _)
-                 (combinational (lut4_and ([i0],[i1],[i2],[i3])%list)))
-      lut4_and_tb_inputs.
+  multistep (Comb lut4_and) lut4_and_tb_inputs.
 
 Definition lut4_and_tb :=
   testBench "lut4_and_tb" lut4_and_Interface
@@ -175,10 +169,7 @@ Definition lut5_and_tb_inputs : list (bool * bool * bool * bool * bool) :=
   (true, true, true, true, true)].
 
 Definition lut5_and_tb_expected_outputs : list bool :=
-  map (fun '(i0,i1,i2,i3,i4) =>
-         List.hd (defaultCombValue _)
-                 (combinational (lut5_and ([i0],[i1],[i2],[i3],[i4])%list)))
-      lut5_and_tb_inputs.
+  multistep (Comb lut5_and) lut5_and_tb_inputs.
 
 Definition lut5_and_tb :=
   testBench "lut5_and_tb" lut5_and_Interface
@@ -207,10 +198,7 @@ Definition lut6_and_tb_inputs : list (bool * bool * bool * bool * bool * bool) :
 
 
 Definition lut6_and_tb_expected_outputs : list bool :=
-  map (fun '(i0,i1,i2,i3,i4,i5) =>
-         List.hd (defaultCombValue _)
-                 (combinational (lut6_and ([i0],[i1],[i2],[i3],[i4],[i5])%list)))
-      lut6_and_tb_inputs.
+  multistep (Comb lut6_and) lut6_and_tb_inputs.
 
 Definition lut6_and_tb :=
   testBench "lut6_and_tb" lut6_and_Interface
